keyshares

src/tls/Negotiation.Writers.Aux.fst
@@ -9,6 +9,9 @@ friend Parsers.ClientHelloExtension_CHE_pre_shared_key
 friend Parsers.PskKeyExchangeModes
 friend Parsers.ClientHelloExtension_CHE_psk_key_exchange_modes
 friend Parsers.ClientHelloExtension_CHE_early_data
+friend Parsers.ServerName
+friend Parsers.NameType
+friend Parsers.ClientHelloExtension_CHE_server_name
 
 module LWP = LowParseWriters.Compat
 module LP = LowParse.Spec
@@ -70,6 +73,8 @@ let valid_offeredPsks_identities_intro =
     )
     _ _
 
+#set-options "--z3rlimit 16"
+
 let valid_offeredPsks_identities_elim =
   let open Parsers.OfferedPsks_identities in
   LWP.valid_rewrite_implies _ _ _ _
@@ -122,3 +127,93 @@ let valid_clientHelloExtension_CHE_psk_key_exchange_modes_intro =
 
 let valid_clientHelloExtension_CHE_early_data_intro =
   LWP.valid_rewrite_parse_bounded_vldata_intro _ _ _ _
+
+inline_for_extraction
+noextract
+let sni_dsum =
+  let open Parsers.ServerName in
+  let open Parsers.UnknownName in
+  let open Parsers.NameType in
+  let open LWP in {
+    dsum_kt = _;
+    dsum_t = serverName_sum;
+    dsum_p = nameType_repr_parser;
+    dsum_s = nameType_repr_serializer;
+    dsum_pc = parse_serverName_cases;
+    dsum_sc = serialize_serverName_cases;
+    dsum_ku = _;
+    dsum_pu = unknownName_parser;
+    dsum_su = unknownName_serializer;
+  }
+
+inline_for_extraction
+noextract
+let sni_enum : LWP.pparser _ _ _ (LP.serialize_maybe_enum_key _ sni_dsum.LWP.dsum_s (LP.dsum_enum sni_dsum.LWP.dsum_t)) =
+  LWP.parse_maybe_enum
+    LWP.parse_u8
+    (LP.dsum_enum sni_dsum.LWP.dsum_t)
+
+let valid_rewrite_constr_sni
+  (k: Parsers.NameType.nameType { LP.list_mem k (LP.list_map fst Parsers.NameType.nameType_enum) })
+  (p: LWP.pparser
+       (Parsers.ServerName.serverName_case_of_nameType k)
+       _
+       (dsnd (Parsers.ServerName.parse_serverName_cases k))
+       (Parsers.ServerName.serialize_serverName_cases k)
+  )
+: Tot (LWP.valid_rewrite_t
+  (Parsers.NameType.lwp_nameType `LWP.parse_pair` p)
+  Parsers.ServerName.lwp_serverName
+  (fun (k', _) -> k' == k)
+  (fun (_, ext) -> Parsers.ServerName.synth_known_serverName_cases k ext)
+)
+=
+  let open Parsers.ServerName in
+  let open Parsers.NameType in
+  let open Parsers.UnknownName in
+  assert_norm (LP.parse_dsum_kind (LP.get_parser_kind nameType_repr_parser) serverName_sum parse_serverName_cases (LP.get_parser_kind unknownName_parser) == serverName_parser_kind);
+  lemma_synth_nameType_inj ();
+  lemma_synth_nameType_inv ();
+  LWP.valid_rewrite_implies _ _ _ _
+  (LWP.valid_rewrite_compose
+    _ _ _ _
+    (LWP.valid_rewrite_parse_pair_compat_r
+      _ _ _ _ _
+      (LWP.valid_rewrite_compose
+        _ _ _ _
+        (LWP.valid_rewrite_parser_eq _ _)
+        _ _ _
+        (LWP.valid_rewrite_parse_synth_recip sni_enum synth_nameType synth_nameType_inv ())
+      )
+    )
+    _ _ _
+    (LWP.valid_rewrite_parse_dsum_known
+      sni_dsum
+      _
+      _
+      k
+      _
+    )
+  )
+  _ _
+
+let valid_rewrite_constr_sni_host_name =
+  let open Parsers.ServerName in
+  let open Parsers.HostName in
+  let open Parsers.NameType in
+  assert_norm (LP.list_mem Host_name (LP.list_map fst nameType_enum) == true);
+  LWP.valid_rewrite_implies _ _ _ _
+    (valid_rewrite_constr_sni Host_name lwp_hostName)
+    _ _
+
+let valid_clientHelloExtension_CHE_server_name_intro =
+  let open Parsers.ClientHelloExtension_CHE_server_name in
+  Classical.forall_intro Parsers.ServerNameList.serverNameList_bytesize_eq;
+  LWP.valid_rewrite_implies _ _ _ _
+    (LWP.valid_rewrite_compose
+      _ _ _ _
+      (LWP.valid_rewrite_parse_synth (LWP.parse_vldata Parsers.ServerNameList.lwp_serverNameList 0ul 65535ul) synth_clientHelloExtension_CHE_server_name synth_clientHelloExtension_CHE_server_name_recip ())
+      _ _ _
+      (LWP.valid_rewrite_parser_eq _ _)
+    )
+  _ _
