src/tls/Negotiation.Writers.Aux2.fsti
@@ -196,3 +196,115 @@ let constr_clientHelloExtension_CHE_early_data'
 = LWP.start Parsers.ExtensionType.lwp_extensionType Parsers.ExtensionType.extensionType_writer Parsers.ExtensionType.Early_data;
   LWP.frame _ _ _ _ _ _ _ (fun _ -> LWP.recast_writer _ _ _ _ _ _ _ f);
   LWP.valid_rewrite _ _ _ _ _ valid_rewrite_constr_clientHelloExtension_CHE_early_data
+
+val valid_rewrite_constr_clientHelloExtension_CHE_key_share : LWP.valid_rewrite_t
+  (Parsers.ExtensionType.lwp_extensionType `LWP.parse_pair` Parsers.ClientHelloExtension.lwp_clientHelloExtension_CHE_key_share)
+  Parsers.ClientHelloExtension.lwp_clientHelloExtension
+  (fun (k, _) -> k == Parsers.ExtensionType.Key_share)
+  (fun (_, ext) -> Parsers.ClientHelloExtension.CHE_key_share ext)
+
+inline_for_extraction
+noextract
+let constr_clientHelloExtension_CHE_key_share
+  #inv #pre #post #post_err
+  ($f: (unit -> LWP.EWrite unit LWP.parse_empty Parsers.ClientHelloExtension.lwp_clientHelloExtension_CHE_key_share pre post post_err inv))
+  ()
+: LWP.EWrite
+    unit
+    LWP.parse_empty
+    Parsers.ClientHelloExtension.lwp_clientHelloExtension
+    (fun _ -> pre ())
+    (fun _ _ msg ->
+      pre () /\
+      begin match LWP.destr_repr_spec _ _ _ _ _ _ _ f () with
+      | LWP.Correct (_, pl) ->
+        post () () pl /\
+        msg == Parsers.ClientHelloExtension.CHE_key_share pl
+      | _ -> False
+      end
+    )
+    (fun _ ->
+      pre () /\
+      begin match LWP.destr_repr_spec _ _ _ _ _ _ _ f () with
+      | LWP.Error _ ->
+        post_err ()
+      | _ -> False
+      end
+    )
+    inv
+= LWP.start Parsers.ExtensionType.lwp_extensionType Parsers.ExtensionType.extensionType_writer Parsers.ExtensionType.Key_share;
+  LWP.frame _ _ _ _ _ _ _ (fun _ -> LWP.recast_writer _ _ _ _ _ _ _ f);
+  LWP.valid_rewrite _ _ _ _ _ valid_rewrite_constr_clientHelloExtension_CHE_key_share
+
+inline_for_extraction
+noextract
+let constr_clientHelloExtension_CHE_key_share'
+  #inv
+  (f: (unit -> LWP.EWrite unit LWP.parse_empty Parsers.ClientHelloExtension.lwp_clientHelloExtension_CHE_key_share (fun _ -> True) (fun _ _ _ -> True) (fun _ -> True) inv))
+: LWP.EWrite
+    unit
+    LWP.parse_empty
+    Parsers.ClientHelloExtension.lwp_clientHelloExtension
+    (fun _ -> True)
+    (fun _ _ msg ->
+      begin match LWP.destr_repr_spec _ _ _ _ _ _ _ f () with
+      | LWP.Correct (_, pl) ->
+        msg == Parsers.ClientHelloExtension.CHE_key_share pl
+      | _ -> False
+      end
+    )
+    (fun _ ->
+      LWP.Error? (LWP.destr_repr_spec _ _ _ _ _ _ _ f ())
+    )
+    inv
+= LWP.start Parsers.ExtensionType.lwp_extensionType Parsers.ExtensionType.extensionType_writer Parsers.ExtensionType.Key_share;
+  LWP.frame _ _ _ _ _ _ _ (fun _ -> LWP.recast_writer _ _ _ _ _ _ _ f);
+  LWP.valid_rewrite _ _ _ _ _ valid_rewrite_constr_clientHelloExtension_CHE_key_share
+
+val valid_rewrite_constr_clientHelloExtension_CHE_server_name : LWP.valid_rewrite_t
+  (Parsers.ExtensionType.lwp_extensionType `LWP.parse_pair` Parsers.ClientHelloExtension.lwp_clientHelloExtension_CHE_server_name)
+  Parsers.ClientHelloExtension.lwp_clientHelloExtension
+  (fun (k, _) -> k == Parsers.ExtensionType.Server_name)
+  (fun (_, ext) -> Parsers.ClientHelloExtension.CHE_server_name ext)
+
+inline_for_extraction
+noextract
+let constr_clientHelloExtension_CHE_server_name'
+  #inv
+  (f: (unit -> LWP.EWrite unit LWP.parse_empty Parsers.ClientHelloExtension.lwp_clientHelloExtension_CHE_server_name (fun _ -> True) (fun _ _ _ -> True) (fun _ -> True) inv))
+: LWP.EWrite
+    unit
+    LWP.parse_empty
+    Parsers.ClientHelloExtension.lwp_clientHelloExtension
+    (fun _ -> True)
+    (fun _ _ msg ->
+      begin match LWP.destr_repr_spec _ _ _ _ _ _ _ f () with
+      | LWP.Correct (_, pl) ->
+        msg == Parsers.ClientHelloExtension.CHE_server_name pl
+      | _ -> False
+      end
+    )
+    (fun _ ->
+      LWP.Error? (LWP.destr_repr_spec _ _ _ _ _ _ _ f ())
+    )
+    inv
+= LWP.start Parsers.ExtensionType.lwp_extensionType Parsers.ExtensionType.extensionType_writer Parsers.ExtensionType.Server_name;
+  LWP.frame _ _ _ _ _ _ _ (fun _ -> LWP.recast_writer _ _ _ _ _ _ _ f);
+  LWP.valid_rewrite _ _ _ _ _ valid_rewrite_constr_clientHelloExtension_CHE_server_name
+
+let rec serverNameList_list_bytesize_correct
+  (l: list Parsers.ServerName.serverName)
+: Lemma
+  (Parsers.ServerNameList.serverNameList_list_bytesize l == LWP.list_size Parsers.ServerName.lwp_serverName l)
+  [SMTPat (Parsers.ServerNameList.serverNameList_list_bytesize l)]
+= match l with
+  | [] -> ()
+  | a :: q ->
+    Parsers.ServerName.serverName_bytesize_eq a;
+    serverNameList_list_bytesize_correct q
+
+val valid_serverNameList_intro : LWP.valid_rewrite_t
+  (LWP.parse_vllist Parsers.ServerName.lwp_serverName 1ul 65535ul)
+  Parsers.ServerNameList.lwp_serverNameList
+  (fun _ -> True)
+  (fun x -> x)
