src/tls/Negotiation.Writers.NoHoare.fst
@@ -24,7 +24,8 @@ let compute_binder_ph1
   ()
 : LWP.TWrite unit LWP.parse_empty lwp_pskBinderEntry inv
 =
-  let c = LWP.deref CipherSuite.cipherSuite13_reader (Parsers.TicketContents13.lwps_accessor_ticketContents13_cs tc) in
+  let cs = Parsers.TicketContents13.lwps_accessor_ticketContents13_cs tc in
+  let c = LWP.deref CipherSuite.cipherSuite13_reader cs in
   let (CipherSuite13 _ h) = cipherSuite_of_cipherSuite13 c in
   let len : U32.t = Hacl.Hash.Definitions.hash_len h in
   LWP.put_vlbytes 32ul 255ul len (Seq.create (U32.v len) 0uy) (fun b ->
@@ -61,11 +62,14 @@ let obfuscate_age1
   ()
 : LWP.TWrite unit LWP.parse_empty Parsers.PskIdentity.lwp_pskIdentity inv
 =
-  LWP.cat (Parsers.ResumeInfo13.lwps_accessor_resumeInfo13_identity ri);
+  let id = Parsers.ResumeInfo13.lwps_accessor_resumeInfo13_identity ri in
+  LWP.cat id;
   let tk = Parsers.ResumeInfo13.lwps_accessor_resumeInfo13_ticket ri in
-  let creation_time = LWP.deref LowParse.Low.Int.read_u32 (Parsers.TicketContents13.lwps_accessor_ticketContents13_creation_time tk) in
+  let ct = Parsers.TicketContents13.lwps_accessor_ticketContents13_creation_time tk in
+  let creation_time = LWP.deref LowParse.Low.Int.read_u32 ct in
   let age = FStar.UInt32.((now -%^ creation_time) *%^ 1000ul) in
-  let age_add = LWP.deref LowParse.Low.Int.read_u32 (Parsers.TicketContents13.lwps_accessor_ticketContents13_age_add tk) in
+  let aa = Parsers.TicketContents13.lwps_accessor_ticketContents13_age_add tk in
+  let age_add = LWP.deref LowParse.Low.Int.read_u32 aa in
   let obfuscated_age = PSK.encode_age age age_add in
   LWP.append LWP.parse_u32 LowParse.Low.Int.write_u32 obfuscated_age;
   LWP.valid_rewrite Aux.valid_pskIdentity_intro'
@@ -243,7 +247,7 @@ let write_binders1
         LWP.list_map
           Parsers.ResumeInfo13.lwp_resumeInfo13
           lwp_pskBinderEntry
-          (fun r -> compute_binder_ph (Parsers.ResumeInfo13.lwps_accessor_resumeInfo13_ticket r))
+          (fun r -> let tk = Parsers.ResumeInfo13.lwps_accessor_resumeInfo13_ticket r in compute_binder_ph tk)
           33ul 65535ul
           lri
           ;
@@ -366,7 +370,9 @@ let write_final_extensions1
     (LWP.parse_vllist Parsers.ClientHelloExtension.lwp_clientHelloExtension 0ul 65535ul)
     (LWP.parse_vllist Parsers.ClientHelloExtension.lwp_clientHelloExtension 0ul 65535ul)
     inv
-= let max_version = LWP.deref Parsers.ProtocolVersion.protocolVersion_reader (Parsers.KnownProtocolVersion.lwps_knownProtocolVersion_accessor_tag (Parsers.MiTLSConfig.lwps_accessor_miTLSConfig_max_version cfg)) in
+= let mv = Parsers.MiTLSConfig.lwps_accessor_miTLSConfig_max_version cfg in
+  let mv = Parsers.KnownProtocolVersion.lwps_knownProtocolVersion_accessor_tag mv in
+  let max_version = LWP.deref Parsers.ProtocolVersion.protocolVersion_reader mv in
   match max_version with
   | TLS_1p3 ->
     let allow_psk_resumption = LWP.list_exists (fun _ -> true) lri in
@@ -418,3 +424,73 @@ let write_final_extensions
     (LWP.parse_vllist Parsers.ClientHelloExtension.lwp_clientHelloExtension 0ul 65535ul)
     inv
 = LWP.wrap_extracted_impl _ _ (extract_write_final_extensions inv cfg edi lri now)
+
+inline_for_extraction
+noextract
+let keyshares1
+  (inv: LWP.memory_invariant)
+  (cfg: LWP.ptr Parsers.MiTLSConfig.lwp_miTLSConfig inv)
+  (ks: option (LWP.ptr lwp_clientHelloExtension_CHE_key_share inv))
+  ()
+: LWP.TWrite unit (LWP.parse_vllist lwp_clientHelloExtension 0ul 65535ul) (LWP.parse_vllist lwp_clientHelloExtension 0ul 65535ul) inv
+=
+  let mv = Parsers.MiTLSConfig.lwps_accessor_miTLSConfig_max_version cfg in
+  let mv = Parsers.KnownProtocolVersion.lwps_knownProtocolVersion_accessor_tag mv in
+  let max_version = LWP.deref Parsers.ProtocolVersion.protocolVersion_reader mv in
+  match max_version, ks with
+  | TLS_1p3, Some ks ->
+    LWP.frame (fun _ -> Aux2.constr_clientHelloExtension_CHE_key_share (fun _ -> LWP.cat ks));
+    LWP.extend_vllist_snoc _ _ _
+  | _ -> ()
+
+noextract
+let keyshares2 = keyshares1
+
+let extract_keyshares
+  (inv: LWP.memory_invariant)
+  (cfg: LWP.ptr Parsers.MiTLSConfig.lwp_miTLSConfig inv)
+  (ks: option (LWP.ptr lwp_clientHelloExtension_CHE_key_share inv))
+: Tot (LWP.extract_t _ (keyshares2 inv cfg ks))
+= LWP.extract _ (keyshares1 _ _ _)
+
+inline_for_extraction
+noextract
+let keyshares
+  (#inv: LWP.memory_invariant)
+  (cfg: LWP.ptr Parsers.MiTLSConfig.lwp_miTLSConfig inv)
+  (ks: option (LWP.ptr lwp_clientHelloExtension_CHE_key_share inv))
+: LWP.TWrite unit (LWP.parse_vllist lwp_clientHelloExtension 0ul 65535ul) (LWP.parse_vllist lwp_clientHelloExtension 0ul 65535ul) inv
+= LWP.wrap_extracted_impl _ _ (extract_keyshares inv cfg ks)
+
+inline_for_extraction
+noextract
+let write_extensions1
+  (inv: LWP.memory_invariant)
+  (cfg: LWP.ptr Parsers.MiTLSConfig.lwp_miTLSConfig inv)
+  (ks: option (LWP.ptr lwp_clientHelloExtension_CHE_key_share inv))
+  (edi: bool)
+  (lri: LWP.lptr Parsers.ResumeInfo13.lwp_resumeInfo13 inv)
+  (now: U32.t)
+  ()
+: LWP.TWrite
+    unit
+    LWP.parse_empty
+    (LWP.parse_vllist Parsers.ClientHelloExtension.lwp_clientHelloExtension 0ul 65535ul)
+    inv
+=
+  LWP.write_vllist_nil _ _;
+  keyshares cfg ks;
+  write_final_extensions cfg edi lri now
+
+noextract
+let write_extensions2 = write_extensions1
+
+let write_extensions
+  (inv: LWP.memory_invariant)
+  (cfg: LWP.ptr Parsers.MiTLSConfig.lwp_miTLSConfig inv)
+  (ks: option (LWP.ptr lwp_clientHelloExtension_CHE_key_share inv))
+  (edi: bool)
+  (lri: LWP.lptr Parsers.ResumeInfo13.lwp_resumeInfo13 inv)
+  (now: U32.t)
+: Tot (LWP.extract_t _ (write_extensions2 inv cfg ks edi lri now))
+= LWP.extract _ (write_extensions1 _ _ _ _ _ _)
